coq: STLC

coq/Logic/STLC/Valid.v
@@ -8,37 +8,14 @@ Require Import Logic.STLC.Context.
 (* ValidVar: Adding a variable declaration with a well-formed type expression   *)
 (* to a valid context yields a valid context.                                   *)
 Inductive Valid (b v:Type) : @Context b v -> Prop :=
-| ValidO   : Valid b v O
-| ValidTy  : forall (G:Context) (t:b),
+| ValidO : Valid b v O
+| ValidT : forall (G:Context) (t:b),
     Valid b v G -> Valid b v (G ; t ::: *)
-| ValidVar : forall (G:Context) (x:v) (Ty:T b),
-    Valid b v G -> G :- Ty -> Valid b v (G ; x ::: Ty) 
+| ValidV : forall (G:Context) (x:v) (Ty:T b),
+    Valid b v G -> G :> Ty -> Valid b v (G ; x ::: Ty) 
 .
 
-Arguments Valid    {b} {v}.
-Arguments ValidO   {b} {v}.
-Arguments ValidTy  {b} {v}.
-Arguments ValidVar {b} {v}.
-
-(* An example of valid context                                                  *)
-(* The variable 'const' is declared with a well-formed type expression.         *)
-Definition G1 (b v:Type) (t t':b) (const:v) : @Context b v 
-    := O
-    ; t  ::: *          (* Type variable declaration                            *)
-    ; t' ::: *          (* Type variable declaration                            *)
-    ; const ::: ((Base t' :-> Base t') :-> Base t :-> Base t' :-> Base t')
-    .
-Arguments G1 {b} {v}.
-
-(* The context G1 is a valid context.                                           *)
-Lemma ValidG1 : forall (b v:Type) (t t':b) (const:v),
-    Valid (G1 t t' const).
-Proof.
-    intros b v t t' const. constructor.
-    - constructor. constructor. constructor.
-    - constructor.
-        + constructor; constructor; apply FindTyZ.
-        + constructor.
-            { constructor. apply FindTyS, FindTyZ. }
-            { constructor; constructor; apply FindTyZ. }
-Qed.
+Arguments Valid  {b} {v}.
+Arguments ValidO {b} {v}.
+Arguments ValidT {b} {v}.
+Arguments ValidV {b} {v}.
