coq/Logic/STLC/Valid2.v
@@ -25,8 +25,8 @@ Inductive Valid2 (b v:Type) : @Context b v -> Prop :=
 with IsType2 (b v:Type) : @Context b v -> T b -> Prop :=
 | TVar2 : forall (G:Context) (t:b),
     Valid2 b v G    ->          (* We require the context to be valid.          *)
-    G :> t          ->
-    IsType2 b v G (Base t)
+    G >> t          ->
+    IsType2 b v G 't
 | TFun2 : forall (G:Context) (Ty Ty':T b),
     Valid2 b v G        ->      (* We require the context to be valid.          *)
     IsType2 b v G Ty    ->
@@ -45,7 +45,7 @@ Arguments TFun2     {b} {v}.
 (* The defining requirements for IsType2 appear to be stronger than those of    *)
 (* IsType, so we expect the implication IsType2 G Ty -> IsType G Ty to hold.    *)
 Lemma IsType2IsType : forall (b v:Type) (G:@Context b v) (Ty:T b),
-    IsType2 G Ty -> G :- Ty.
+    IsType2 G Ty -> G :> Ty.
 Proof.
    intros b v G Ty H1. induction H1 as [G Ty H2 H3|G Ty Ty' H2 H3 IH1 H4 IH2]. 
    - constructor. assumption.
@@ -66,7 +66,7 @@ Qed.
 (* We cannot expect the implication IsType G Ty -> IsType2 G Ty to hold, but    *)
 (* this is however true if the context involved is 'strongly' valid.            *)
 Lemma IsTypeIsType2 : forall (b v:Type) (G:@Context b v) (Ty:T b),
-    Valid2 G -> G :- Ty -> IsType2 G Ty.
+    Valid2 G -> G :> Ty -> IsType2 G Ty.
 Proof.
     intros b v G Ty H H1. revert H.
     induction H1 as [G t|G Ty Ty' H2 IH1 H3 IH2].
@@ -80,7 +80,7 @@ Qed.
 (* This is the main helper lemma: the conclusion of this lemma needs to be      *)
 (* strong enough so we are able to carry out the induction argument.            *)
 Lemma ValidValid2IsType2 : forall (b v:Type) (G:@Context b v),
-    Valid G -> Valid2 G /\ (forall (Ty:T b), G :- Ty -> IsType2 G Ty).
+    Valid G -> Valid2 G /\ (forall (Ty:T b), G :> Ty -> IsType2 G Ty).
 Proof.
     intros b v G H1. induction H1 as [ |G t H2 IH|G x Ty H2 IH H3].
     - split; try constructor. intros Ty H2. 
@@ -98,7 +98,7 @@ Qed.
 (* This is a strenghening of the IsTypeIsType2 result, where we can now rely    *)
 (* on the weaker assumption that the context is simply valid (not 'strongly').  *)
 Lemma IsTypeIsType2' : forall (b v:Type) (G:@Context b v) (Ty:T b),
-    Valid G -> G :- Ty -> IsType2 G Ty.
+    Valid G -> G :> Ty -> IsType2 G Ty.
 Proof.
     intros b v G Ty H1 H2. apply ValidValid2IsType2 in H1.
     destruct H1 as [H1 H3]. apply H3. assumption.
