coq/Logic/STLC/Context.v
@@ -11,11 +11,11 @@ Arguments Binding {b} {v}.
 Arguments BType   {b} {v}.
 Arguments BVar    {b} {v}.
 
-Notation "Ty ::: *" := (BType Ty)
+Notation "t ::: *" := (BType t)
     (at level 1, no associativity)      : STLC_Context_scope.
 
 Notation "x ::: Ty" :=(BVar x Ty)
-    (at level 1, no associativity)      : STLC_Context_scope.
+    (at level 5, no associativity)      : STLC_Context_scope.
 
 
 Inductive Context (b v:Type) : Type :=
@@ -32,21 +32,21 @@ Notation "G ; x" := (CtxSnoc G x)
 
 Open Scope STLC_Context_scope.
 
-Inductive FindTy (b v:Type) : @Context b v -> b -> Prop :=
-| FindTyZ : forall (G:Context) (t:b), FindTy b v (G ; t ::: *) t
-| FindTyS : forall (G:Context) (t:b) (k:Binding),
-    FindTy b v G t -> FindTy b v (G ; k) t
+Inductive FindT (b v:Type) : @Context b v -> b -> Prop :=
+| FindTZ : forall (G:Context) (t:b), FindT b v (G ; t ::: *) t
+| FindTS : forall (G:Context) (t:b) (k:Binding),
+    FindT b v G t -> FindT b v (G ; k) t
 .
 
-Arguments FindTy  {b} {v}.
-Arguments FindTyZ {b} {v}.
-Arguments FindTyS {b} {v}.
+Arguments FindT  {b} {v}.
+Arguments FindTZ {b} {v}.
+Arguments FindTS {b} {v}.
 
-Notation "G :> Ty" := (FindTy G Ty)
+Notation "G >> t" := (FindT G t)
     (at level 60, no associativity) : STLC_Context_scope.
 
-Lemma findTyRev : forall (b v:Type) (G:Context) (x:v) (Ty:T b) (t : b),
-    G ; x ::: Ty :> t -> G :> t.
+Lemma findTRev : forall (b v:Type) (G:Context) (x:v) (Ty:T b) (t : b),
+    G ; x ::: Ty >> t -> G >> t.
 Proof.
     intros b v G x Ty t H1. remember (G ; x ::: Ty) as G' eqn:E.
     revert G x Ty E. destruct H1 as [G t|G t k H1]; intros G' x Ty H2.
@@ -54,8 +54,8 @@ Proof.
     - inversion H2. subst. assumption.
 Qed.
 
-Lemma findTyRev' : forall (b v:Type) (G:@Context b v) (t t':b),
-    G ; t ::: * :> t' -> t = t' \/ G :> t'.
+Lemma findTRev' : forall (b v:Type) (G:@Context b v) (t t':b),
+    G ; t ::: * >> t' -> t = t' \/ G >> t'.
 Proof.
     intros b v G t t' H1. remember (G;t ::: *) as G' eqn:E.
     revert G t E. destruct H1 as [G t|G t k H2];
@@ -64,26 +64,26 @@ Proof.
     - subst. right. assumption.
 Qed.
 
-Inductive FindVar (b v:Type) (e:Eq v) : @Context b v -> @Binding b v -> Prop :=
-| FindVarZ : forall (G:Context) (x:v) (Ty:T b), 
-    FindVar b v e (G ; x ::: Ty) (x ::: Ty)
-| FindVarSkip : forall (G:Context) (k:Binding) (t:b),
-    FindVar b v e G k -> FindVar b v e (G ; t ::: * ) k
-| FindVarS : forall (G:Context) (x y:v) (Ty Ty':T b),
-    x <> y                                      ->
-    FindVar b v e G (x ::: Ty)                  ->
-    FindVar b v e (G ; y ::: Ty') (x ::: Ty)
+Inductive FindV (b v:Type) (e:Eq v) : @Context b v -> @Binding b v -> Prop :=
+| FindVZ : forall (G:Context) (x:v) (Ty:T b), 
+    FindV b v e (G ; x ::: Ty) (x ::: Ty)
+| FindVK : forall (G:Context) (k:Binding) (t:b),
+    FindV b v e G k -> FindV b v e (G ; t ::: * ) k
+| FindVS : forall (G:Context) (x y:v) (Ty Ty':T b),
+    x <> y                                  ->
+    FindV b v e G (x ::: Ty)                ->
+    FindV b v e (G ; y ::: Ty') (x ::: Ty)
 .
 
-Arguments FindVar     {b} {v} {e}.
-Arguments FindVarZ    {b} {v} {e}.
-Arguments FindVarSkip {b} {v} {e}.
-Arguments FindVarS    {b} {v} {e}.
+Arguments FindV  {b} {v} {e}.
+Arguments FindVZ {b} {v} {e}.
+Arguments FindVK {b} {v} {e}.
+Arguments FindVS {b} {v} {e}.
 
-Notation "G :>> k" := (FindVar G k)
+Notation "G :>> k" := (FindV G k)
     (at level 60, no associativity) : STLC_Context_scope.
 
-Lemma findVarRev : forall (b v:Type) (e:Eq v) (G:Context) (t:b) (x:v) (Ty:T b),
+Lemma findVRev : forall (b v:Type) (e:Eq v) (G:Context) (t:b) (x:v) (Ty:T b),
     G ; t ::: * :>> x ::: Ty -> G :>> x ::: Ty.
 Proof.
     intros b v e G t x Ty H1.
@@ -96,7 +96,7 @@ Proof.
 Qed.
 
 Definition ctxIncl (b v:Type)(e:Eq v)(G H:@Context b v) : Prop :=
-    (forall (t:b), G :> t -> H :> t) /\
+    (forall (t:b), G >> t -> H >> t) /\
     (forall (x:v) (Ty:T b), G :>> x ::: Ty -> H :>> x ::: Ty).
 
 Arguments ctxIncl {b} {v} {e}.
@@ -132,24 +132,24 @@ Proof.
     intros b v e G H t [H1 H2]. split.
     - intros t' H3.  remember (G ; t ::: * ) as G' eqn:E.
       revert G H H1 H2 t E. destruct H3 as [G t|G t k H1].
-        + intros G' H H2 H3 t' H4. inversion H4. apply FindTyZ.
+        + intros G' H H2 H3 t' H4. inversion H4. apply FindTZ.
         + intros G' H H2 H3 t' H4. inversion H4. subst.
-          apply FindTyS, H2. assumption.
-    - intros x t' H3. constructor. apply H2. apply findVarRev in H3. assumption.
+          apply FindTS, H2. assumption.
+    - intros x t' H3. constructor. apply H2. apply findVRev in H3. assumption.
 Qed.
 
 Lemma ctxInclExtendVar : forall (b v:Type)(e:Eq v)(G H:@Context b v)(x:v)(Ty:T b),
     G <= H -> G ; x ::: Ty <= H ; x ::: Ty.
 Proof.
     intros b v e G H x Ty [H1 H2]. split.
-    - intros Sy H3. apply FindTyS, H1. apply findTyRev in H3. assumption.
+    - intros Sy H3. apply FindTS, H1. apply findTRev in H3. assumption.
     - intros x' Ty' H3.
       remember (G ; x ::: Ty) as G' eqn:E. remember (x' ::: Ty') as k eqn:F.
       revert G H x Ty H1 H2 x' Ty' E F.
       destruct H3 as [G x Ty|G k Ty H1|G x y Ty Sy H1 H2];
       intros G' H x' Ty' H3 H4 y' Sy' H5 H6. 
-        + inversion H5. apply FindVarZ.
+        + inversion H5. apply FindVZ.
         + inversion H5.
-        + inversion H5. subst. apply FindVarS; try assumption. 
+        + inversion H5. subst. apply FindVS; try assumption. 
           apply H4. assumption.
 Qed.
