coq/Logic/STLC/Example.v
@@ -5,8 +5,12 @@ Require Import Logic.Class.Eq.
 Require Import Logic.STLC.Eval.
 Require Import Logic.STLC.Value.
 Require Import Logic.STLC.Subst.
+Require Import Logic.STLC.Valid.
+Require Import Logic.STLC.IsType.
+Require Import Logic.STLC.Typing.
 Require Import Logic.STLC.Syntax.
 Require Import Logic.STLC.Replace.
+Require Import Logic.STLC.Context.
 
 Definition id (b v:Type)(x:v) : Exp b v := \x ~> `x.
 
@@ -19,7 +23,7 @@ Arguments const {b} {v}.
 
 (* Annotated identity applied to variable y reduces to variable y               *)
 Lemma idAnn : forall (b v:Type) (e:Eq v) (x y:v) (Ty:T b),
-    (id x :: Ty :-> Ty) $ `y >> `y.
+    (id x :: Ty :-> Ty) $ `y >>> `y.
 Proof.
     intros b v e x y Ty. apply (EAppL (id x :: Ty :-> Ty) `x _ _ x).
     - apply VVar.
@@ -33,7 +37,8 @@ Qed.
 (* Annotated const applied to identity and variable u reduces to identity       *)
 (* Note that we need the variables x and y to be distinct for this to hold      *)
 Lemma constAnn : forall (b v:Type) (e:Eq v) (x y z u:v) (Ty Ty' : T b),
-    x <> y -> (const x y :: (Ty' :-> Ty') :-> Ty :-> Ty' :-> Ty') $ (id z) $ `u >> id z. 
+    x <> y -> 
+    (const x y :: (Ty' :-> Ty') :-> Ty :-> Ty' :-> Ty') $ (id z) $ `u >>> id z. 
 Proof.
     intros base v e x y z u Ty Ty' H1. apply (EAppL _ (id z) _ _ y).
     - apply VLam, VVar.
@@ -62,4 +67,94 @@ Proof.
         + destruct (in_dec eqDec z (z :: nil)) as [H2|H2].
             { apply EVar. }
             { exfalso. apply H2. left. reflexivity. }
+Qed.
+
+(* An example of valid context.                                                 *)
+Lemma Valid1 : forall (b v:Type) (t t':b) (x:v),
+    Valid   ( O 
+            ; t  ::: * 
+            ; t' ::: * 
+            ; x  ::: (('t' :-> 't') :-> 't :-> 't' :-> 't')
+            ).
+Proof.
+    intros b v t t' x. apply ValidV.
+    - apply ValidT, ValidT, ValidO.
+    - apply TFun.
+        + apply TFun; apply TVar, FindTZ.
+        + apply TFun.
+            { apply TVar, FindTS, FindTZ. }
+            { apply TFun; apply TVar, FindTZ. }
+Qed.
+
+Lemma Typing1 : forall (b v:Type)(eq:Eq v)(t:b)(x y:v),
+    O ; t ::: * ; y ::: 't :- (id x :: 't :-> 't) $ `y >: 't.
+Proof.
+    intros b v eq t x y. apply JApp with 't.
+    - apply JAnn, JLam.
+        + apply ValidV.
+            { apply ValidT, ValidO. }
+            { apply TVar, FindTZ. }
+        + apply TVar, FindTS, FindTZ.
+        + apply JVar.
+            { apply ValidV.
+                { apply ValidV.
+                    { apply ValidT, ValidO. }
+                    { apply TVar, FindTZ. }}
+                { apply TVar, FindTS, FindTZ. }}
+            { apply FindVZ. }
+    - apply JVar.
+        + apply ValidV.
+            { apply ValidT, ValidO. }
+            { apply TVar, FindTZ. }
+        + apply FindVZ.
+Qed.
+
+Lemma Typing2 : forall (b v:Type) (eq:Eq v) (t t':b) (x y z u:v),
+    x <> y ->
+        O ; t ::: * ; u ::: 't ; t' ::: * 
+            :-
+        (const x y :: ('t' :-> 't') :-> 't :-> 't' :-> 't') $ (id z) $ `u
+            >:
+        't' :-> 't'.
+Proof.
+    intros b v eq t t' x y z u H1. apply JApp with 't.
+    - apply JApp with ('t' :-> 't').
+        + apply JAnn, JLam.
+            { apply ValidT, ValidV.
+                { apply ValidT, ValidO. }
+                { apply TVar, FindTZ. }}
+            { apply TFun; apply TVar, FindTZ. }
+            { apply JLam.
+                { apply ValidV.
+                    { apply ValidT, ValidV. 
+                        { apply ValidT, ValidO. }
+                        { apply TVar, FindTZ. }}
+                    { apply TFun; apply TVar, FindTZ. }}
+                { apply TVar, FindTS, FindTS, FindTS, FindTZ. }
+                { apply JVar.
+                    { apply ValidV.
+                        { apply ValidV.
+                            { apply ValidT, ValidV.
+                                { apply ValidT, ValidO. }
+                                { apply TVar, FindTZ. }}
+                            { apply TFun; apply TVar, FindTZ. }}
+                        { apply TVar, FindTS, FindTS, FindTS, FindTZ. }}
+                    { apply FindVS; try assumption. apply FindVZ. }}}
+        + apply JLam.
+            { apply ValidT, ValidV.
+                { apply ValidT, ValidO. }
+                { apply TVar, FindTZ. }}
+            { apply TVar, FindTZ. }
+            { apply JVar.
+                { apply ValidV.
+                    { apply ValidT, ValidV.
+                        { apply ValidT, ValidO. }
+                        { apply TVar, FindTZ. }}
+                    { apply TVar, FindTZ. }}
+                { apply FindVZ. }}
+    - apply JVar.
+        + apply ValidT, ValidV.
+            { apply ValidT, ValidO. }
+            { apply TVar, FindTZ. }
+        + apply FindVK, FindVZ.
 Qed.
