coq/Logic/STLC/Typing.v
@@ -20,8 +20,6 @@ Open Scope STLC_Typing_scope.
 
 Inductive Judgement (b v:Type) (eq:Eq v): @Context b v -> @Typing b v  -> Prop :=
 | JAnn : forall (G:Context) (e:Exp b v) (Ty:T b),
-    Valid G                                 ->  (* G is a valid context         *)
-    G :- Ty                                 ->  (* Ty well-formed expression    *)
     Judgement b v eq G (e >: Ty)            ->  (* e is of type Ty in context G *) 
     Judgement b v eq G ((e :: Ty) >: Ty)        (* Annotated expr same type     *)
 | JVar : forall (G:Context) (x:v) (Ty:T b),
@@ -29,8 +27,23 @@ Inductive Judgement (b v:Type) (eq:Eq v): @Context b v -> @Typing b v  -> Prop :
     G :>> x ::: Ty                          ->  (* variable x declared type Ty  *) 
     Judgement b v eq G (`x >: Ty)               (* variable expr same type      *) 
 | JApp : forall (G:Context) (e1 e2:Exp b v) (Ty Ty':T b),
-    Valid G                                 ->  (* G is a valid context         *)
     Judgement b v eq G (e1 >: Ty :-> Ty')   ->  (* e1 of type Ty :-> Ty'        *)
     Judgement b v eq G (e2 >: Ty)           ->  (* e2 of type Ty                *)
     Judgement b v eq G (e1 $ e2 >: Ty')         (* e1 e2 of type Ty'            *)
+| JLam : forall (G:Context) (x:v) (Ty Ty':T b) (e:Exp b v),
+    Valid G                                 ->  (* G is a valid context         *)
+    G :> Ty                                 ->  (* Ty well-formed expression    *)
+    Judgement b v eq (G;x ::: Ty) (e >: Ty')->  (* e is of type Ty' with x:::Ty *)
+    Judgement b v eq G ((\x ~> e) >: Ty :-> Ty')(* \x -> e is of type Ty :-> Ty'*)
 .
+
+Arguments Judgement {b} {v} {eq}.
+Arguments JAnn      {b} {v} {eq}.
+Arguments JVar      {b} {v} {eq}.
+Arguments JApp      {b} {v} {eq}.
+Arguments JLam      {b} {v} {eq}.
+
+Notation "G :- T" := (Judgement G T)
+    (at level 90, no associativity) : STLC_Typing_scope.
+
+Open Scope STLC_Typing_scope.
